more changes to indexing

examples/crypto/HyE.PlainAE.fst
@@ -3,57 +3,60 @@ module HyE.PlainAE
 open CoreCrypto
 open HyE.Flags
 open HyE.Indexing
-//open HyE.PlainHPKE
+open HyE.PlainHPKE
 open Platform.Bytes
+
 
 (**
    The content of the AE payload depends on the honesty of the message.
    If it is an honest message, it encapsulates a (protected) hpke payload.
    If it is not an honest message, it is plain bytes.
 *)
-
-//TODO: Not sure if/how this works. This module should not have to import PlainHPKE.
-//assume type ae_plain_content (i:ae_id) 
-//assume val ae_content_length: #i:ae_id -> ae_plain_content i -> Tot nat
-
-//= (
-//  if honest i && hpke_ind_cca then
-//    p:protected_hpke_plain{get_index p = _,i}
-//  else 
-//    hpke_plain
-//  )
+noeq abstract type protected_ae_plain (i:ae_id) = (
+  if pke_honest (fst i) && not ae_honest i && hpke_ind_cca then
+    p:protected_hpke_plain (fst i)
+  else 
+    hpke_plain
+  )
 
 type ae_plain = Bytes.bytes
 
-noeq abstract type protected_ae_plain (i:ae_id)=
-  | Protected_ae_plain: (p:ae_plain) -> protected_ae_plain i
-
 val length: #i:ae_id -> (protected_ae_plain i) -> Tot nat
 let length #i p = 
-    Bytes.length p.p
+  if ae_honest i && hpke_ind_cca then
+    PlainHPKE.length p.p
+  else
+    length p.p
 
 (**
    Coerced messages can only be flagged as not honest.
 *)
 val coerce: #i:ae_id -> p:ae_plain{not ae_ind_cca || not (ae_honest i)} -> Tot (protected_ae_plain i)
 let coerce #i p = 
-  Protected_ae_plain #i p
+  p
 
 (**
    We allow a transition from protected_ae_plain to ae_plain only if either there is no
    idealization or if if the message is not honest.
 *)
-val repr: #i:ae_id -> p:protected_ae_plain i{not ae_ind_cca || not (ae_honest i)} -> Tot (ae_plain)
+val repr: #i:ae_id -> p:protected_ae_plain i{not ae_ind_cca || not (ae_honest i)} -> Tot (ae_plain_content i)
 let repr #i p = 
-  p.p
+  if ae_honest i && ae_ind_cca then
+    PlainHPKE.repr p.p 
+  else
+    p.p
+
 (**
    This is a helper function used by HPKE.encrypt to encapsulate the payload before
    passing it on to AE.encrypt. If AE is idealized and the payload is honest, then we 
    wrap the payload into our abstract type in good faith. If not, we coerce it.
 *)
-val ae_message_wrap: #i:ae_id -> p:ae_plain{ae_honest i && ae_ind_cca} -> Tot (protected_ae_plain i)
+val ae_message_wrap: #i:ae_id -> p:ae_plain_content i -> Tot (protected_ae_plain i)
 let ae_message_wrap #i p =
+  if ae_honest i && ae_ind_cca then
     Protected_ae_plain p
+  else
+    coerce p
 
 (**
    This is the reverse function to ae_message_wrap. HPKE.decrypt uses it to extract a
@@ -61,10 +64,10 @@ let ae_message_wrap #i p =
    we strip it of its protection in good faith. Otherwise we break it down to its 
    byte representation using repr.
 *)
-val ae_message_unwrap: #i:ae_id -> p:protected_ae_plain i -> Tot (ae_plain)
+val ae_message_unwrap: #i:ae_id -> p:protected_ae_plain i -> Tot (ae_plain_content i)
 let ae_message_unwrap #i p =
   if ae_honest i && ae_ind_cca then
     p.p
   else 
-    repr p
-  
+repr p
+
