examples/crypto/HyE.PlainHPKE.fst
@@ -10,13 +10,11 @@ open Platform.Bytes
 
 open HyE.Flags
 open HyE.Indexing
-open HyE.PlainAE
 
 type hpke_plain = Bytes.bytes
 
 abstract type protected_hpke_plain (i:pke_id)= 
   | Prot_hpke_p: b:hpke_plain -> protected_hpke_plain i
-//assume Plain_hasEq: hasEq protected_hpke_plain
 
 (* two pure functions, never called when ideal *)
 val repr: #i:pke_id -> p:protected_hpke_plain i{not (pke_honest i) || not hpke_ind_cca} -> Tot (hpke_plain)
@@ -26,16 +24,6 @@ let repr #i p = p.b
 val coerce: #i:pke_id -> p:hpke_plain{not (pke_honest i) || not hpke_ind_cca} -> Tot (protected_hpke_plain i)
 let coerce #i p = 
   Prot_hpke_p #i p
-
-val hpke_message_wrap: #pk_id:pke_id 
-		     -> #k_id:ae_id 
-		     -> p:protected_hpke_plain pk_id{
-			 pke_honest pk_id && 
-			 ae_honest k_id &&
-			 hpke_ind_cca}
-		     -> Tot (protected_ae_plain k_id)
-let hpke_message_wrap #pk_id #k_id p =
-  PlainAE.ae_message_wrap #k_id p.b
 
 val length: #i:pke_id -> protected_hpke_plain i -> Tot nat
 let length #i p = Bytes.length p.b
